Repr.LV
A representation using linear variables

pure/Learn.List.Mask.fst
@@ -1,25 +1,42 @@
 module Learn.List.Mask
 
-module T = FStar.Tactics
+module T    = FStar.Tactics
+module Perm = Learn.Permutation
+
+
+#push-options "--ifuel 1 --fuel 1"
+
+let rec mask_not_len (#n : nat) ($mask : vec n bool)
+  : Lemma (ensures mask_len (mask_not mask) = n - mask_len mask) (decreases n)
+          [SMTPat (mask_len (mask_not mask))]
+  = match mask with
+  | [] -> ()
+  | _ :: mask -> mask_not_len (mask <: vec (n-1) bool)
 
 let rec merge_fun_on_mask_index #src_n mask #b f g (i : nat)
   : Lemma (requires i < src_n)
           (ensures  index (merge_fun_on_mask #src_n mask #b f g) i ==
-                   (if index mask i then f i (mask_push #src_n mask i) else g i))
+                   (if index mask i then f i (mask_push mask i) else g i (mask_push (mask_not mask) i)))
           [SMTPat (index (merge_fun_on_mask #src_n mask #b f g) i)]
   = match mask with
   | true  :: mask ->
-          let f' (i : Fin.fin (src_n-1) {index mask i}) (j : Fin.fin (mask_len mask)) = f (i + 1) (j + 1) in
-          let g' (i : Fin.fin (src_n-1) {not (index mask i)}) = g (i + 1) in
+          let mask : vec (src_n-1) bool = mask in
+          let f' (i : Fin.fin (src_n-1) {     index mask i }) (j : Fin.fin (mask_len           mask))
+            = f (i + 1) (j + 1) in
+          let g' (i : Fin.fin (src_n-1) {not (index mask i)}) (j : Fin.fin (mask_len (mask_not mask)))
+            = g (i + 1)    j    in
           assert (merge_fun_on_mask #src_n (true :: mask) f g ==
                   f 0 0 :: merge_fun_on_mask #(src_n-1) mask f' g')
               by (T.trefl ());
           if i > 0 then merge_fun_on_mask_index #(src_n-1) mask f' g' (i - 1)
   | false :: mask ->
-          let f' (i : Fin.fin (src_n-1) {index mask i}) (j : Fin.fin (mask_len mask)) = f (i + 1) j in
-          let g' (i : Fin.fin (src_n-1) {not (index mask i)}) = g (i + 1) in
+          let mask : vec (src_n-1) bool = mask in
+          let f' (i : Fin.fin (src_n-1) {     index mask i }) (j : Fin.fin (mask_len           mask))
+            = f (i + 1)    j    in
+          let g' (i : Fin.fin (src_n-1) {not (index mask i)}) (j : Fin.fin (mask_len (mask_not mask)))
+            = g (i + 1) (j + 1) in
           assert (merge_fun_on_mask #src_n (false :: mask) f g ==
-                  g 0 :: merge_fun_on_mask #(src_n-1) mask f' g')
+                  g 0 0 :: merge_fun_on_mask #(src_n-1) mask f' g')
               by (T.trefl ());
           if i > 0 then merge_fun_on_mask_index #(src_n-1) mask f' g' (i - 1)
 
@@ -63,6 +80,138 @@ let rec filter_mask_true (#a : Type) (#len : nat) (mask : vec len bool) (l : vec
   = match mask, l with
   | [], [] -> ()
   | b :: mask, x :: xs -> tr 0; filter_mask_true #a #(len-1) mask xs (fun i -> tr (i+1))
+
+let rec filter_mask_false (#a : Type) (#len : nat) (mask : vec len bool) (l : vec len a)
+      (fl : (i : Fin.fin len) -> squash (not (index mask i)))
+  : Lemma (ensures filter_mask mask l == []) (decreases mask)
+  = match mask, l with
+  | [], [] -> ()
+  | b :: mask, x :: xs -> fl 0; filter_mask_false #a #(len-1) mask xs (fun i -> fl (i+1))
+
+
+let rec mask_comp_or_index
+      (#len : nat)
+      (m0 : vec len bool)
+      (m1 : vec (mask_len (mask_not m0)) bool)
+      (i : Fin.fin len)
+  : Lemma (ensures   index (mask_comp_or m0 m1) i == (index m0 i || index m1 (mask_push (mask_not m0) i)))
+          (decreases len)
+          [SMTPat (index (mask_comp_or m0 m1) i)]
+  = match m0, m1 with
+  | [], []  -> ()
+  | true  :: m0, m1 | false :: m0, _  :: m1 ->
+      if i > 0 then mask_comp_or_index #(len-1) m0 m1 (i-1)
+
+let rec mask_comp_or_assoc #len m0 m1 m2
+  : Lemma (ensures   mask_comp_or (mask_comp_or m0 m1) m2 == mask_comp_or m0 (mask_comp_or m1 m2))
+          (decreases m0)
+  = match m0, m1, m2 with
+  | [], [], [] -> ()
+  | true  :: m0, m1, m2 | false :: m0, true  :: m1, m2 | false :: m0, false :: m1, _ :: m2 ->
+      mask_comp_or_assoc #(len-1) m0 m1 m2
+
+let rec mask_not_comp_or #len m0 m1
+  : Lemma (ensures   mask_not (mask_comp_or m0 m1) == mask_comp_and (mask_not m0) (mask_not m1))
+          (decreases m0)
+  = match m0, m1 with
+  | [], [] -> ()
+  | true :: m0, m1 | false :: m0, _ :: m1 -> mask_not_comp_or #(len-1) m0 m1
+
+let rec filter_mask_and #a #len m0 m1 l
+  : Lemma (ensures filter_mask (mask_comp_and m0 m1) l == filter_mask m1 (filter_mask m0 l))
+          (decreases m0)
+  = match m0, m1, l with
+  | [], [], [] -> ()
+  | true :: m0, _ :: m1, _ :: l | false :: m0, m1, _ :: l -> filter_mask_and #a #(len-1) m0 m1 l
+
+
+let tac_filter_mask_or () : T.Tac unit = T.(
+  norm [delta_only [`%mask_or_append_f]; zeta];
+  norm [iota];
+  norm [delta_only [`%U.cast]; iota])
+
+#push-options "--z3rlimit 20"
+
+let rec filter_mask_or_append
+      (#a : Type) (#len : nat) (m0 : vec len bool) (m1 : vec (mask_len (mask_not m0)) bool) (l : vec len a)
+  : Tot (squash (filter_mask m0 l @ filter_mask m1 (filter_mask (mask_not m0) l)
+              == Perm.apply_perm_r (mask_or_append_f m0 m1) (filter_mask (mask_comp_or m0 m1) l)))
+        (decreases len)
+  = match m0, m1, l with
+  | [], [], [] -> ()
+  | true :: m0', m1, x :: xs ->
+      let m0' : vec (len-1) bool = m0'    in
+      let lhs = filter_mask m0' xs @ filter_mask m1 (filter_mask (mask_not m0') xs) in
+      let rhs = filter_mask (mask_comp_or m0' m1) xs in
+      assert (x :: lhs == Perm.apply_perm_r (mask_or_append_f #len (true :: m0') m1) (x :: rhs))
+        by T.(tac_filter_mask_or ();
+              apply (`Perm.pequiv_cons_eq); smt ();
+                apply (`filter_mask_or_append))
+  | false :: m0', true :: m1', x :: xs ->
+      let m0' : vec (len-1) bool = m0' in
+      let lhs0 = filter_mask m0' xs in
+      let lhs1 = filter_mask m1' (filter_mask (mask_not m0') xs) in
+      let rhs  = filter_mask (mask_comp_or m0' m1') xs in
+      assert (filter_mask m0 l @ filter_mask m1 (filter_mask (mask_not m0) l) == lhs0 @ x :: lhs1);
+      assert (Perm.apply_perm_r (mask_or_append_f m0 m1) (filter_mask (mask_comp_or m0 m1) l)
+           == Perm.apply_perm_r (mask_or_append_f #len (false :: m0') (true :: m1')) (x :: rhs));
+      assert (lhs0 @ x :: lhs1 == Perm.apply_perm_r (mask_or_append_f #len (false :: m0') (true :: m1')) (x :: rhs))
+        by T.(tac_filter_mask_or ();
+              apply (`Perm.pequiv_trans_eq); later ();
+                apply_raw (`Perm.pequiv_cons_eq); later (); later ();
+                  apply_raw (`filter_mask_or_append);
+                apply_raw (`Perm.pequiv_move_head_eq); later ();
+              explode (); trefl (); iterAll smt)
+  | false :: m0, false :: m1, x :: xs ->
+      let m0 : vec (len-1) bool = m0 in
+      filter_mask_or_append m0 m1 xs
+
+(*
+[@@__mask__]
+let rec filter_mask_or_append
+      (#a : Type) (#len : nat) (m0 : vec len bool) (m1 : vec (mask_len (mask_not m0)) bool) (l : vec len a)
+  : Tot (Perm.pequiv (filter_mask (mask_comp_or m0 m1) l)
+                     (filter_mask m0 l @ filter_mask m1 (filter_mask (mask_not m0) l)))
+        (decreases len)
+  = match m0, m1, l with
+  | [], [], [] ->
+      U.cast _ (Perm.pequiv_refl #a [])
+  | true :: m0, m1, x :: xs ->
+      let m0 : vec (len-1) bool = m0 in
+      U.cast _ (Perm.pequiv_cons x (filter_mask_or_append m0 m1 xs))
+  | false :: m0, true :: m1, x :: xs ->
+      let m0 : vec (len-1) bool = m0 in
+      U.cast _ Perm.(pequiv_trans #_ #_ #_ #(filter_mask m0 xs @ x :: filter_mask m1 (filter_mask (mask_not m0) xs))
+          (pequiv_cons x (filter_mask_or_append m0 m1 xs))
+          (pequiv_move_head x (filter_mask m0 xs) (filter_mask m1 (filter_mask (mask_not m0) xs))))
+  | false :: m0, false :: m1, x :: xs ->
+      let m0 : vec (len-1) bool = m0 in
+      U.cast _ (filter_mask_or_append m0 m1 xs)
+  | _ -> false_elim () // avoids ifuel
+*)
+
+[@@__mask__]
+let rec filter_mask_or_append'
+      (#a : Type) (#len : nat) (m0 : vec len bool) (m1 : vec (mask_len (mask_not m0)) bool) (l : vec len a)
+  : Tot (Perm.pequiv (filter_mask m0 l @ filter_mask m1 (filter_mask (mask_not m0) l))
+                     (filter_mask (mask_comp_or m0 m1) l))
+        (decreases len)
+  = match m0, m1, l with
+  | [], [], [] ->
+      U.cast _ (Perm.pequiv_refl #a [])
+  | true :: m0, m1, x :: xs ->
+      let m0 : vec (len-1) bool = m0 in
+      U.cast _ (Perm.pequiv_cons x (filter_mask_or_append' #a #(len-1) m0 m1 xs))
+  | false :: m0, true :: m1, x :: xs ->
+      let m0 : vec (len-1) bool = m0 in
+      U.cast _ Perm.(pequiv_trans #_ #_ #_ #(x :: filter_mask (mask_comp_or m0 m1) xs)
+          (pequiv_move_to_head x (filter_mask m0 xs) (filter_mask m1 (filter_mask (mask_not m0) xs)))
+          (pequiv_cons x (filter_mask_or_append' #a #(len-1) m0 m1 xs)))
+  | false :: m0, false :: m1, x :: xs ->
+      let m0 : vec (len-1) bool = m0 in
+      U.cast _ (filter_mask_or_append' m0 m1 xs)
+#pop-options
+
 
 let rec filter_mask_dl_index (#len : nat) (mask : vec len bool) (ts : vec len Type) (xs : Dl.dlist ts) (i : nat)
   : Lemma (requires i < mask_len mask)
