pure/Learn.List.Mask.fsti
@@ -1,9 +1,10 @@
 module Learn.List.Mask
 
-module U   = Learn.Util
-module Dl  = Learn.DList
-module Fl  = Learn.FList
-module Fin = FStar.Fin
+module U    = Learn.Util
+module Dl   = Learn.DList
+module Fl   = Learn.FList
+module Fin  = FStar.Fin
+module Perm = Learn.Permutation
 
 open FStar.List.Pure
 open Learn.List
@@ -11,12 +12,20 @@ open Learn.List
 
 irreducible let __mask__ : unit = ()
 
+type mask_t (#a : Type) (l : list a) =
+  vec (length l) bool
+
 [@@__mask__]
 let mask_len (mask : list bool) : nat =
   count true mask
 
+[@@__mask__]
 let mask_not (#n : nat) ($mask : vec n bool) : vec n bool
   = map not mask
+
+val mask_not_len (#n : nat) ($mask : vec n bool)
+  : Lemma (mask_len (mask_not mask) = n - mask_len mask)
+          [SMTPat (mask_len (mask_not mask))]
 
 [@@__mask__]
 let rec filter_mask (#a : Type) (#len : nat) (mask : vec len bool) (l : vec len a)
@@ -42,24 +51,47 @@ let rec mask_pull (#len : nat) (mask : vec len bool) (j : Fin.fin (mask_len mask
   | true  :: mask -> if j = 0 then 0 else 1 + mask_pull #(len - 1) mask (j - 1)
   | false :: mask -> 1 + mask_pull #(len - 1) mask j
 
+
+[@@__mask__]
+let rec mask_comp_and (#len : nat) (m0 : vec len bool) (m1 : vec (mask_len m0) bool)
+  : Pure (vec len bool) (requires True) (ensures fun m -> mask_len m = mask_len m1) (decreases m0)
+  = match m0 with
+  | [] -> []
+  | true  :: m0 -> let hd1 :: m1 = m1 in
+                 hd1 :: mask_comp_and #(len-1) m0 m1
+  | false :: m0 -> false :: mask_comp_and #(len-1) m0 m1
+
+[@@__mask__]
+let rec mask_comp_or (#len : nat) (m0 : vec len bool) (m1 : vec (mask_len (mask_not m0)) bool)
+  : Pure (vec len bool) (requires True) (ensures fun m -> mask_len m = mask_len m0 + mask_len m1) (decreases m0)
+  = match m0 with
+  | [] -> []
+  | true  :: m0 -> true :: mask_comp_or #(len-1) m0 m1
+  | false :: m0 -> let hd1 :: m1 = m1 in
+                 hd1 :: mask_comp_or #(len-1) m0 m1
+
+
 (* TODO? optimize *)
 [@@__mask__]
 let rec merge_fun_on_mask (#src_n : nat) (mask : vec src_n bool) (#b : Type)
-      (f : (i : Fin.fin src_n {index mask i}) -> (j : Fin.fin (mask_len mask)) -> b)
-      (g : (i : Fin.fin src_n {not (index mask i)}) -> b)
+      (f : (i : Fin.fin src_n {     index mask i }) -> (j : Fin.fin (mask_len            mask)) -> b)
+      (g : (i : Fin.fin src_n {not (index mask i)}) -> (j : Fin.fin (mask_len (mask_not mask))) -> b)
   : Tot (vec src_n b) (decreases mask)
   = match mask with
   | [] -> []
-  | true  :: mask -> f 0 0 :: merge_fun_on_mask #(src_n-1) mask (fun i j -> f (i+1) (j+1)) (fun i -> g (i+1))
-  | false :: mask -> g 0   :: merge_fun_on_mask #(src_n-1) mask (fun i j -> f (i+1)   j  ) (fun i -> g (i+1))
+  | true  :: mask -> f 0 0 :: merge_fun_on_mask (mask <: vec (src_n-1) bool)
+                            (fun i j -> f (i+1) (j+1)) (fun i j -> g (i+1)   j  )
+  | false :: mask -> g 0 0 :: merge_fun_on_mask (mask <: vec (src_n-1) bool)
+                            (fun i j -> f (i+1)   j  ) (fun i j -> g (i+1) (j+1))
 
 
 val merge_fun_on_mask_index (#src_n : nat) (mask : vec src_n bool) (#b : Type)
-      (f : (i : Fin.fin src_n {index mask i}) -> (j : Fin.fin (mask_len mask)) -> b)
-      (g : (i : Fin.fin src_n {not (index mask i)}) -> b) (i : nat)
+      (f : (i : Fin.fin src_n {     index mask i }) -> (j : Fin.fin (mask_len            mask)) -> b)
+      (g : (i : Fin.fin src_n {not (index mask i)}) -> (j : Fin.fin (mask_len (mask_not mask))) -> b)
+      (i : nat)
   : Lemma (requires i < src_n)
           (ensures  index (merge_fun_on_mask #src_n mask #b f g) i ==
-                   (if index mask i then f i (mask_push #src_n mask i) else g i))
+                   (if index mask i then f i (mask_push mask i) else g i (mask_push (mask_not mask) i)))
           [SMTPat (index (merge_fun_on_mask #src_n mask #b f g) i)]
 
 val mask_push_pull (#len : nat) (mask : vec len bool) (j : Fin.fin (mask_len mask))
@@ -93,6 +125,58 @@ val filter_mask_true (#a : Type) (#len : nat) (mask : vec len bool) (l : vec len
       (tr : (i : Fin.fin len) -> squash (index mask i))
   : Lemma (filter_mask mask l == l)
 
+val filter_mask_false (#a : Type) (#len : nat) (mask : vec len bool) (l : vec len a)
+      (fl : (i : Fin.fin len) -> squash (not (index mask i)))
+  : Lemma (filter_mask mask l == [])
+
+
+val mask_comp_or_index
+      (#len : nat)
+      (m0 : vec len bool)
+      (m1 : vec (mask_len (mask_not m0)) bool)
+      (i : Fin.fin len)
+  : Lemma (index (mask_comp_or m0 m1) i == (index m0 i || index m1 (mask_push (mask_not m0) i)))
+          [SMTPat (index (mask_comp_or m0 m1) i)]
+
+val mask_comp_or_assoc
+      (#len : nat)
+      (m0 : vec len bool)
+      (m1 : vec (mask_len (mask_not m0)) bool)
+      (m2 : vec (mask_len (mask_not (mask_comp_or m0 m1 <: vec len bool))) bool)
+  : Lemma (mask_comp_or (mask_comp_or m0 m1) m2 == mask_comp_or m0 (mask_comp_or m1 m2))
+
+val mask_not_comp_or
+      (#len : nat) (m0 : vec len bool) (m1 : vec (mask_len (mask_not m0)) bool)
+  : Lemma (mask_not (mask_comp_or m0 m1) == mask_comp_and (mask_not m0) (mask_not m1))
+
+val filter_mask_and
+      (#a : Type) (#len : nat) (m0 : vec len bool) (m1 : vec (mask_len m0) bool) (l : vec len a)
+  : Lemma (filter_mask (mask_comp_and m0 m1) l == filter_mask m1 (filter_mask m0 l))
+
+
+#push-options "--ifuel 1 --fuel 1"
+let rec mask_or_append_f (#len : nat) (m0 : vec len bool) (m1 : vec (mask_len (mask_not m0)) bool)
+  : Tot (Perm.perm_f (mask_len (mask_comp_or m0 m1))) (decreases m0)
+  = match m0, m1 with
+  | [], [] ->
+      U.cast _ Perm.(id_n 0)
+  | true :: m0, m1 ->
+      let m0 : vec (len-1) bool = m0 in
+      U.cast _ Perm.(perm_f_cons (mask_or_append_f #(len-1) m0 m1))
+  | false :: m0, true :: m1 ->
+      let m0 : vec (len-1) bool = m0 in
+      U.cast _ Perm.(comp
+          (perm_f_move_head (mask_len m0) (mask_len m1))
+          (U.cast _ (perm_f_cons (mask_or_append_f #(len-1) m0 m1))))
+  | false :: m0, false :: m1 ->
+      let m0 : vec (len-1) bool = m0 in
+      U.cast _ (mask_or_append_f m0 m1)
+#pop-options
+
+val filter_mask_or_append
+      (#a : Type) (#len : nat) (m0 : vec len bool) (m1 : vec (mask_len (mask_not m0)) bool) (l : vec len a)
+  : squash (filter_mask m0 l @ filter_mask m1 (filter_mask (mask_not m0) l)
+         == Perm.apply_perm_r (mask_or_append_f m0 m1) (filter_mask (mask_comp_or m0 m1) l))
 
 [@@__mask__]
 let rec filter_mask_dl (#len : nat) (mask : vec len bool) (ts : vec len Type) (xs : Dl.dlist ts)
