experiment/Experiment.Steel.Repr.LV.fst
@@ -1,0 +1,266 @@
+module Experiment.Steel.Repr.LV
+
+module Perm = Learn.Permutation
+
+open FStar.List.Pure
+open Learn.List.Mask
+open FStar.Tactics
+
+
+let bind_g_csm'_len
+      (env : vprop_list)
+      (f_csm : csm_t env) (f_prd : vprop_list)
+      (g_csm : csm_t (filter_mask (mask_not f_csm) env))
+  : Lemma (mask_len (bind_g_csm' env f_csm f_prd g_csm) == length f_prd + mask_len g_csm)
+          [SMTPat (mask_len (bind_g_csm' env f_csm f_prd g_csm))]
+  =
+    append_count (Ll.repeat (length f_prd) true) g_csm true;
+    Ll.repeat_count (length f_prd) true true
+
+#push-options "--ifuel 0"
+let rec bind_g_csm'_or_aux
+      (n m : nat) (f : Ll.vec m bool) (g : Ll.vec (mask_len (mask_not f)) bool)
+  : Lemma (ensures  (append_count (Ll.repeat n true) f true; Ll.repeat_count n true true;
+                     mask_comp_or #(n+m) (Ll.repeat n true @ f) g == Ll.repeat n true @ mask_comp_or f g))
+          (decreases n)
+  = if n > 0 then begin
+      append_count (Ll.repeat   n   true) f true; Ll.repeat_count   n   true true;
+      bind_g_csm'_or_aux (n-1) m f g
+    end
+#pop-options
+
+let bind_g_csm'_or
+      (env : vprop_list)
+      (f_csm : csm_t env) (f_prd : vprop_list)
+      (g_csm : csm_t (filter_mask (mask_not f_csm) env))
+      (csm1  : csm_t (filter_mask (mask_not g_csm) (filter_mask (mask_not f_csm) env)))
+  : Lemma (mask_comp_or (bind_g_csm' env f_csm f_prd g_csm) csm1
+        == bind_g_csm' env f_csm f_prd (mask_comp_or g_csm csm1))
+  =
+    bind_g_csm'_or_aux (length f_prd) (mask_len (mask_not f_csm)) g_csm csm1
+
+#push-options "--ifuel 0 --fuel 0"
+
+let filter_bind_csm
+      (env : vprop_list)
+      (f_csm : csm_t env)
+      (g_csm : csm_t (filter_mask (mask_not f_csm) env))
+  : Lemma (filter_mask (mask_not (bind_csm env f_csm g_csm)) env
+        == filter_mask (mask_not g_csm) (filter_mask (mask_not f_csm) env))
+  =
+    mask_not_comp_or f_csm g_csm;
+    filter_mask_and (mask_not f_csm) (mask_not g_csm) env
+
+let filter_bind_g_csm'
+      (env : vprop_list)
+      (f_csm : csm_t env) (f_prd : vprop_list)
+      (g_csm : csm_t (filter_mask (mask_not f_csm) env))
+  : Lemma (filter_mask (mask_not (bind_g_csm' env f_csm f_prd g_csm)) (res_env env f_csm f_prd)
+        == filter_mask (mask_not (bind_csm env f_csm g_csm)) env)
+  =
+    let env1 = filter_mask (mask_not f_csm) env in
+    let m1 : Ll.vec (length f_prd + mask_len (mask_not f_csm)) bool
+      = Ll.repeat (length f_prd) true @ g_csm in
+    let m2 : Ll.vec (length f_prd + mask_len (mask_not f_csm)) bool
+      = Ll.repeat (length f_prd) false @ mask_not g_csm in
+    calc (==) {
+      filter_mask (mask_not (bind_g_csm' env f_csm f_prd g_csm)) (res_env env f_csm f_prd) <: vprop_list;
+    == { }
+      filter_mask (mask_not m1) (f_prd @ env1);
+    == { Ll.pat_append () }
+      filter_mask m2 (f_prd @ env1);
+    == { filter_mask_append (Ll.repeat (length f_prd) false) (mask_not g_csm) f_prd env1 }
+      filter_mask (Ll.repeat (length f_prd) false) f_prd @ filter_mask (mask_not g_csm) env1;
+    == { filter_mask_false (Ll.repeat (length f_prd) false) f_prd (fun _ -> ()) }
+      [] @ filter_mask (mask_not g_csm) env1;
+    == { _ by (Tactics.trefl ()) }
+      filter_mask (mask_not g_csm) env1;
+    == { filter_bind_csm env f_csm g_csm }
+      filter_mask (mask_not (bind_csm env f_csm g_csm)) env;
+    }
+#pop-options
+
+(**) private let __end_bind_lem = ()
+
+#set-options "--ifuel 0 --fuel 0"
+
+let sub_ret_prd_f_eij
+      (#env : vprop_list)
+      (#prd0 : vprop_list) (csm_f0 : eq_injection_l prd0 env)
+      (#csm1 : csm_t (filter_mask (mask_not (eij_trg_mask csm_f0)) env)) (#prd1 : vprop_list)
+      (prd_f1 : vequiv_perm (sub_prd env (eij_trg_mask csm_f0) prd0 csm1) prd1)
+  : Lemma (is_eq_injection prd1 env (sub_ret_prd_f' csm_f0 prd_f1))
+  =
+    (**) Ll.pat_append ();
+    let n0    = length prd0 in
+    let ncsm0 = mask_not (eij_trg_mask csm_f0) in
+    let f = sub_ret_prd_f' csm_f0 prd_f1 in
+    (**) assert (eq_injection_eq prd1 env f);
+    Perm.injectiveI #(Fin.fin (length prd1)) f (fun i i' ->
+      let j  = f i       in
+      let k  = prd_f1 i  in
+      let k' = prd_f1 i' in
+
+      U.assert_by (k == k') (fun () ->
+        if k < n0 && k' < n0
+        then assert (index csm_f0 k == index csm_f0 k') // then injectivity of csm_f0
+        else if k >= n0 && k' >= n0
+        then // by injectivity of mask_pull
+          assert (
+             mask_push csm1 (mask_push ncsm0 (mask_pull ncsm0 (mask_pull csm1 (k - n0))))
+          ==
+             mask_push csm1 (mask_push ncsm0 (mask_pull ncsm0 (mask_pull csm1 (k' - n0)))))
+        else if k < n0 && k' >= n0
+        then begin
+          assert (index ncsm0 j);      // by k'
+          assert (~(mem j csm_f0));    // definition of [eij_trg_mask]
+          assert (j = index csm_f0 k); // since k < n0
+          lemma_index_memP csm_f0 k;
+          false_elim ()
+        end else begin
+          assert (k >= n0 && k' < n0);
+          assert (~(mem j csm_f0));
+          lemma_index_memP csm_f0 k';
+          false_elim ()
+        end);
+      Perm.perm_f_injective prd_f1
+    )
+
+#push-options "--z3rlimit 20"
+let sub_ret_prd_f_eij_trg_eq
+      (#env : vprop_list)
+      (#prd0 : vprop_list) (csm_f0 : eq_injection_l prd0 env)
+      (#csm1 : csm_t (filter_mask (mask_not (eij_trg_mask csm_f0)) env)) (#prd1 : vprop_list)
+      (prd_f1 : vequiv_perm (sub_prd env (eij_trg_mask csm_f0) prd0 csm1) prd1)
+  : Lemma (bind_csm env (eij_trg_mask csm_f0) csm1 == eij_trg_mask (sub_ret_prd_f csm_f0 (prd_f1)))
+  = Ll.list_extensionality
+      (bind_csm env (eij_trg_mask csm_f0) csm1) (eij_trg_mask (sub_ret_prd_f csm_f0 (prd_f1)))
+    (fun j ->
+        let n0    = length prd0 in
+        let csm0  = eij_trg_mask csm_f0 in
+        let ncsm0 = mask_not csm0 in
+        calc (==) {
+          index (bind_csm env csm0 csm1) j;
+        == { }
+          index (mask_comp_or csm0 csm1) j;
+        == { mask_comp_or_index csm0 csm1 j }
+          index csm0 j || index csm1 (mask_push ncsm0 j);
+        };
+        calc (<==>) {
+          b2t (index (eij_trg_mask (sub_ret_prd_f csm_f0 (prd_f1))) j);
+        <==> { }
+          memP j (sub_ret_prd_f csm_f0 (prd_f1));
+        <==> { Ll.memP_iff j (sub_ret_prd_f csm_f0 (prd_f1)) }
+          exists (i : Fin.fin (length prd1)) . index (sub_ret_prd_f csm_f0 (prd_f1)) i == j;
+        <==> { }
+          exists (i : Fin.fin (length prd1)) .
+            (let k = prd_f1 i in
+             if k < n0 then index csm_f0 k else (mask_pull ncsm0 (mask_pull csm1 (k - n0)))) == j;
+        <==> { introduce forall (k : Fin.fin (length (sub_prd env csm0 prd0 csm1))) . exists (i : Fin.fin (length prd1)) .
+                         k = prd_f1 i
+               with assert Perm.(prd_f1 (inv_f prd_f1 k) == (prd_f1 `comp` inv_f prd_f1) k) }
+          exists (k : Fin.fin (length (sub_prd env csm0 prd0 csm1))) .
+            (if k < n0 then index csm_f0 k else (mask_pull ncsm0 (mask_pull csm1 (k - n0)))) == j;
+        <==> { introduce forall (k' : Fin.fin (mask_len csm1)) .
+                       exists (k : Fin.fin (length (sub_prd env csm0 prd0 csm1))) .
+                         k' = k - n0
+               with assert (k' = (k'+n0) - n0) }
+             (exists (k : Fin.fin n0) . index csm_f0 k == j)
+          \/ (exists (k : Fin.fin (mask_len csm1)) .
+                (mask_pull ncsm0 (mask_pull csm1 k)) == j);
+        <==> { Ll.memP_iff j csm_f0 }
+          index csm0 j \/ (exists (k : Fin.fin (mask_len csm1)) . (mask_pull csm1 k == mask_push ncsm0 j));
+        <==> { introduce forall (j' : Fin.fin (mask_len ncsm0)) .
+                 (exists (k : Fin.fin (mask_len csm1)) . mask_pull csm1 k == j') <==> index csm1 j'
+               with assert (index csm1 j' ==> (mask_pull csm1 (mask_push csm1 j')) == j') }
+          index csm0 j \/ index csm1 (mask_push ncsm0 j);
+        }
+      )
+#pop-options
+
+
+#push-options "--ifuel 1 --fuel 0 --z3rlimit 20"
+(**) private let ___begin_lc_sub_push = ()
+
+
+let norm_lcsbl (norm_atlv : bool) : Tac unit =
+      norm [delta_only [`%lc_sub_push; `%lc_sub_push_aux;
+                        `%lcsubp_LCret; `%lcsubp_LCbind; `%lcsubp_LCsub]; iota; zeta];
+      if norm_atlv then (norm [delta_only [`%lcsub_at_leaves]; zeta]; norm [iota])
+
+let rew_lcsub_at_leaves_csm
+      (#env : vprop_list) (#a : Type u#a) (#t : M.prog_tree a) (#csm : csm_t env) (#prd : prd_t a)
+      (ct : lin_cond env t csm prd)
+      (csm' : csm_t env)
+      (pf : squash (lcsub_at_leaves #env #a #t #csm #prd ct))
+      (_ : squash (csm == csm'))
+  : squash (lcsub_at_leaves #env #a #t #csm' #prd ct)
+  = pf
+
+// TODO? use t_destruct
+
+#push-options "--ifuel 1 --fuel 1"
+let rec lc_sub_push_at_leaves
+      (env : vprop_list) (#a : Type u#a) (#t : M.prog_tree a) (#csm : csm_t env) (#prd : prd_t a)
+      (ct : lin_cond env t csm prd)
+  : Lemma (ensures lcsub_at_leaves (lc_sub_push ct)) (decreases %[ct; 1])
+  = match ct with
+  | LCspec _ _ | LCret  _ _ _ -> ()
+  | LCbind env f_csm f_prd cf g_csm g_prd cg ->
+      assert (lcsub_at_leaves (lc_sub_push (LCbind env f_csm f_prd cf g_csm g_prd cg)))
+          by (norm_lcsbl true;
+              split ();
+                apply_lemma (``@lc_sub_push_at_leaves);
+                let _ = forall_intro () in apply_lemma (``@lc_sub_push_at_leaves))
+  | LCsub  env csm prd cf csm' prd' prd_f ->
+      lc_sub_push_aux_at_leaves _ cf csm' prd' prd_f
+
+and lc_sub_push_aux_at_leaves
+      (env : vprop_list) (#a0 : Type u#a) (#t0 : M.prog_tree a0) (#csm0 : csm_t env) (#prd0 : prd_t a0)
+      (ct0 : lin_cond env t0 csm0 prd0)
+      (csm'0 : csm_t (filter_mask (mask_not csm0) env)) (prd'0 : prd_t a0)
+      (prd_f0 : ((x : a0) -> Perm.pequiv_list (sub_prd env csm0 (prd0 x) csm'0) (prd'0 x)))
+  : Lemma (ensures lcsub_at_leaves (lc_sub_push_aux ct0 csm'0 prd'0 prd_f0)) (decreases %[ct0; 0])
+  =
+    let goal #a #t #csm #prd ct csm' prd' prd_f =
+      lcsub_at_leaves (lc_sub_push_aux #env #a #t #csm #prd ct csm' prd' prd_f) in
+    match_lin_cond ct0
+      (fun a t csm prd ct ->
+         (csm' : csm_t (filter_mask (mask_not csm) env)) -> (prd' : prd_t a) ->
+         (prd_f : ((x : a) -> Perm.pequiv_list (sub_prd env csm (prd x) csm') (prd' x))) ->
+         squash (goal ct csm' prd' prd_f))
+    begin fun (*LCspec*) a pre post req ens csm_f -> fun csm' prd' prd_f ->
+      assert (goal (LCspec env #a #pre #post #req #ens csm_f) csm' prd' prd_f)
+          by (norm_lcsbl true; trivial ())
+    end
+    begin fun (*LCret*)  a x sl_hint prd csm_f -> fun csm' prd' prd_f ->
+      assert (goal (LCret env #a #x #sl_hint prd csm_f) csm' prd' prd_f)
+          by (norm_lcsbl true; trivial ())
+    end
+    begin fun (*LCbind*) a b f g f_csm f_prd cf g_csm g_prd cg -> fun csm' prd' prd_f ->
+      // Some guards generated by the tactic
+      let gd0 : squash (L.length csm' =
+                        L.length (filter_mask (mask_not g_csm) (filter_mask (mask_not f_csm) env)))
+              = filter_bind_csm env f_csm g_csm in
+      let gd1 (x : a) : squash (L.length csm' =
+                        L.length (filter_mask (mask_not (bind_g_csm' env f_csm (f_prd x) g_csm))
+                                              (res_env env f_csm (f_prd x))))
+              = filter_bind_g_csm' env f_csm (f_prd x) g_csm in
+      FStar.Classical.forall_intro_squash_gtot gd1;
+      assert (goal (LCbind env #a #b #f #g f_csm f_prd cf g_csm g_prd cg) csm' prd' prd_f)
+          by (norm_lcsbl true;
+              split ();
+                apply_lemma (`lc_sub_push_at_leaves);
+                let _ = forall_intro () in
+                  apply (`rew_lcsub_at_leaves_csm);
+                  apply_lemma (`lc_sub_push_aux_at_leaves);
+                  apply_lemma (`bind_g_csm'_or))
+    end
+    begin fun (*LCsub*)  a f csm0 prd0 cf csm1 prd1 prd_f1 -> fun csm2 prd2 prd_f2 ->
+      assert (goal (LCsub env #a #f csm0 prd0 cf csm1 prd1 prd_f1) csm2 prd2 prd_f2)
+          by (norm_lcsbl false;
+              apply (`rew_lcsub_at_leaves_csm);
+              apply_lemma (`lc_sub_push_aux_at_leaves);
+              smt ())
+    end csm'0 prd'0 prd_f0
+#pop-options
