experiment/Experiment.Steel.Repr.LV.fsti
@@ -1,0 +1,572 @@
+module Experiment.Steel.Repr.LV
+
+module U    = Learn.Util
+module L    = FStar.List.Pure
+module M    = Experiment.Steel.Repr.M
+module Ll   = Learn.List
+module Fl   = Learn.FList
+module Perm = Learn.Permutation
+
+open Learn.List.Mask
+open Experiment.Steel.VPropList
+
+
+type csm_t (env : vprop_list) = mask_t env
+type prd_t (a : Type) = a -> vprop_list
+
+type req_t (env : vprop_list) = sl_f env -> Type0
+type ens_t (env : vprop_list) (a : Type) (prd : prd_t a) = sl_f env -> (x : a) -> sl_f (prd x) -> Type0
+
+let res_env (env : vprop_list) (csm : csm_t env) (prd : vprop_list) : vprop_list =
+  L.(prd @ (filter_mask (mask_not csm) env))
+
+let res_sel (#env : vprop_list) (sl0 : sl_f env) (csm : csm_t env) (#prd : vprop_list) (sl1 : sl_f prd)
+  : sl_f (res_env env csm prd)
+  =
+    (**) Ll.pat_append ();
+    Fl.append sl1 (filter_mask_fl (mask_not csm) (vprop_list_sels_t env) sl0)
+
+
+(****** [eq_injection] *)
+
+type eq_injection' (#a : Type) (src trg : list a) =
+  Fin.fin (L.length src) -> Fin.fin (L.length trg)
+  
+let eq_injection_eq (#a : Type) (src trg : list a) (f : eq_injection' src trg) : prop
+  = forall (i : Fin.fin (L.length src)) . L.index trg (f i) == L.index src i
+
+let is_eq_injection (#a : Type) (src trg : list a) (f : eq_injection' src trg) : prop
+  = Perm.injective f /\ eq_injection_eq src trg f
+
+type eq_injection (#a : Type) (src trg : list a) =
+  f : eq_injection' src trg { is_eq_injection src trg f }
+
+type eq_injection_l (#a : Type) (src trg : list a) =
+  l : Ll.vec (L.length src) (Fin.fin (L.length trg)) { is_eq_injection src trg (L.index l) }
+
+let eij_trg_mask_f (#a : Type) (#src #trg : list a) (eij : eq_injection_l src trg) (j : Fin.fin (L.length trg))
+  : bool
+  = L.mem j eij
+
+let eij_trg_mask (#a : Type) (#src #trg : list a) (eij : eq_injection_l src trg)
+  : Ll. vec (L.length trg) bool
+  = Ll.initi 0 (L.length trg) (eij_trg_mask_f eij)
+
+let eij_sl (#src #trg : vprop_list) (eij : eq_injection src trg) (xs : sl_f trg)
+  : sl_f src
+  = Fl.mk_flist (vprop_list_sels_t src) (fun i -> xs (eij i) <: (L.index src i).t)
+
+
+(*** [lin_cond] *)
+
+let bind_g_csm'
+      (env : vprop_list)
+      (f_csm : csm_t env) (f_prd : vprop_list)
+      (g_csm : csm_t (filter_mask (mask_not f_csm) env))
+  : csm_t (res_env env f_csm f_prd)
+  = L.(Ll.repeat (length f_prd) true @ g_csm)
+
+let bind_csm
+      (env : vprop_list)
+      (f_csm : csm_t env)
+      (g_csm : csm_t (filter_mask (mask_not f_csm) env))
+  : csm_t env
+  = mask_comp_or f_csm g_csm
+
+val bind_g_csm'_len
+      (env : vprop_list)
+      (f_csm : csm_t env) (f_prd : vprop_list)
+      (g_csm : csm_t (filter_mask (mask_not f_csm) env))
+  : Lemma (mask_len (bind_g_csm' env f_csm f_prd g_csm) == L.length f_prd + mask_len g_csm)
+          [SMTPat (mask_len (bind_g_csm' env f_csm f_prd g_csm))]
+
+val bind_g_csm'_or
+      (env : vprop_list)
+      (f_csm : csm_t env) (f_prd : vprop_list)
+      (g_csm : csm_t (filter_mask (mask_not f_csm) env))
+      (csm1  : csm_t (filter_mask (mask_not g_csm) (filter_mask (mask_not f_csm) env)))
+  : Lemma (mask_comp_or (bind_g_csm' env f_csm f_prd g_csm) csm1
+        == bind_g_csm' env f_csm f_prd (mask_comp_or g_csm csm1))
+
+val filter_bind_csm
+      (env : vprop_list)
+      (f_csm : csm_t env)
+      (g_csm : csm_t (filter_mask (mask_not f_csm) env))
+  : Lemma (filter_mask (mask_not (bind_csm env f_csm g_csm)) env
+        == filter_mask (mask_not g_csm) (filter_mask (mask_not f_csm) env))
+
+val filter_bind_g_csm'
+      (env : vprop_list)
+      (f_csm : csm_t env) (f_prd : vprop_list)
+      (g_csm : csm_t (filter_mask (mask_not f_csm) env))
+  : Lemma (filter_mask (mask_not (bind_g_csm' env f_csm f_prd g_csm)) (res_env env f_csm f_prd)
+        == filter_mask (mask_not (bind_csm env f_csm g_csm)) env)
+
+(**) private val __end_bind_lem : unit
+
+let sub_prd
+      (env : vprop_list)
+      (csm : csm_t env) (prd : vprop_list)
+      (csm' : csm_t (filter_mask (mask_not csm) env))
+  : vprop_list
+  = L.(prd @ filter_mask csm' (filter_mask (mask_not csm) env))
+
+
+noeq
+type lin_cond : 
+     (env : vprop_list) ->
+     (#a : Type u#a) -> (t : M.prog_tree a) ->
+     (csm : csm_t env) -> (prd : prd_t a) ->
+     Type u#(max (a+1) 2)
+  =
+  | LCspec :
+      (env : vprop_list) ->
+      (#a : Type u#a) -> (#pre : M.pre_t) -> (#post : M.post_t a) ->
+      (#req : M.req_t pre) -> (#ens : M.ens_t pre a post) ->
+      (csm_f : eq_injection_l pre env) ->
+      lin_cond env (M.Tspec a pre post req ens) (eij_trg_mask csm_f) post
+  | LCret :
+      (env : vprop_list) ->
+      (#a : Type u#a) -> (#x : a) -> (#sl_hint : M.post_t a) ->
+      (prd : prd_t a) -> (csm_f : eq_injection_l (prd x) env) ->
+      lin_cond env (M.Tret a x sl_hint) (eij_trg_mask csm_f) prd
+  | LCbind :
+      (env : vprop_list) ->
+      (#a : Type u#a) -> (#b : Type u#a) -> (#f : M.prog_tree a) -> (#g : (a -> M.prog_tree b)) ->
+      (f_csm : csm_t env) -> (f_prd : prd_t a) ->
+      (cf : lin_cond env f f_csm f_prd) ->
+      // [g_csm] and [g_prd] are independent of the return value [x : a] of [f]
+      (g_csm : csm_t (filter_mask (mask_not f_csm) env)) -> (g_prd : prd_t b) ->
+      (cg : ((x : a) ->
+        lin_cond (res_env env f_csm (f_prd x)) (g x) (bind_g_csm' env f_csm (f_prd x) g_csm) g_prd)) ->
+      lin_cond env (M.Tbind a b f g) (bind_csm env f_csm g_csm) g_prd
+  | LCsub :
+      (env : vprop_list) -> (#a : Type u#a) -> (#f : M.prog_tree a) ->
+      (csm : csm_t env) -> (prd : prd_t a) ->
+      (cf : lin_cond env f csm prd) ->
+      (csm' : csm_t (filter_mask (mask_not csm) env)) -> (prd' : prd_t a) ->
+      (prd_f : ((x : a) -> Perm.pequiv_list (sub_prd env csm (prd x) csm') (prd' x))) ->
+      lin_cond env f (bind_csm env csm csm') prd'
+
+
+unfold
+let match_lin_cond
+      (#env : vprop_list)
+      (#a0 : Type u#a) (#t0 : M.prog_tree a0)
+      (#csm0 : csm_t env) (#prd0 : prd_t a0)
+      (ct0 : lin_cond env t0 csm0 prd0)
+      (r : (a : Type u#a) -> (t : M.prog_tree a) -> (csm : csm_t env) -> (prd : prd_t a) ->
+           (ct : lin_cond env t csm prd) -> Type u#r)
+      (c_LCspec : (a : Type u#a) -> (pre : M.pre_t) -> (post : M.post_t a) ->
+                  (req : M.req_t pre) -> (ens : M.ens_t pre a post) ->
+                  (csm_f : eq_injection_l pre env) ->
+                  Pure (r _ _ _ _ (LCspec env #a #pre #post #req #ens csm_f))
+                       (requires a0 == a /\ t0 == M.Tspec a pre post req ens /\
+                                 csm0 == eij_trg_mask csm_f /\ prd0 == post /\
+                                 ct0 == LCspec env #a #pre #post #req #ens csm_f)
+                       (ensures fun _ -> True))
+      (c_LCret  : (a : Type u#a) -> (x : a) -> (sl_hint : M.post_t a) ->
+                  (prd : prd_t a) -> (csm_f : eq_injection_l (prd x) env) ->
+                  Pure (r _ _ _ _ (LCret env #a #x #sl_hint prd csm_f))
+                       (requires a0 == a /\ t0 == M.Tret a x sl_hint /\
+                                 csm0 == eij_trg_mask csm_f /\ prd0 == prd /\
+                                 ct0 == LCret env #a #x #sl_hint prd csm_f)
+                       (ensures fun _ -> True))
+      (c_LCbind : (a : Type u#a) -> (b : Type u#a) -> (f : M.prog_tree a) -> (g : (a -> M.prog_tree b)) ->
+                  (f_csm : csm_t env) -> (f_prd : prd_t a) ->
+                  (cf : lin_cond env f f_csm f_prd {cf << ct0}) ->
+                  (g_csm : csm_t (filter_mask (mask_not f_csm) env)) -> (g_prd : prd_t b) ->
+                  (cg : ((x : a) ->
+                        lin_cond (res_env env f_csm (f_prd x)) (g x)
+                                 (bind_g_csm' env f_csm (f_prd x) g_csm) g_prd)
+                        {forall (x : a) . {:pattern (cg x)} cg x << ct0}) ->
+                  Pure (r _ _ _ _ (LCbind env #a #b #f #g f_csm f_prd cf g_csm g_prd cg))
+                       (requires a0 == b /\ t0 == M.Tbind a b f g /\
+                                 csm0 == bind_csm env f_csm g_csm /\ prd0 == g_prd /\
+                                 ct0 == LCbind env #a #b #f #g f_csm f_prd cf g_csm g_prd cg)
+                       (ensures fun _ -> True))
+      (c_LCsub  : (a : Type u#a) -> (f : M.prog_tree a) ->
+                  (csm : csm_t env) -> (prd : prd_t a) ->
+                  (cf : lin_cond env f csm prd {cf << ct0}) ->
+                  (csm' : csm_t (filter_mask (mask_not csm) env)) -> (prd' : prd_t a) ->
+                  (prd_f : ((x : a) -> Perm.pequiv_list (sub_prd env csm (prd x) csm') (prd' x))) ->
+                  Pure (r _ _ _ _ (LCsub env #a #f csm prd cf csm' prd' prd_f))
+                       (requires a0 == a /\ t0 == f /\
+                                 csm0 == bind_csm env csm csm' /\ prd0 == prd' /\
+                                 ct0 == LCsub env #a #f csm prd cf csm' prd' prd_f)
+                       (ensures fun _ -> True))
+  : r _ _ _ _ ct0
+  = match ct0 as ct returns r _ _ _ _ ct with
+  | LCspec env #a #pre #post #req #ens csm_f             -> c_LCspec a pre post req ens csm_f
+  | LCret  env #a #x #sl_hint prd csm_f                  -> c_LCret  a x sl_hint prd csm_f
+  | LCbind env #a #b #f #g f_csm f_prd cf g_csm g_prd cg -> c_LCbind a b f g f_csm f_prd cf g_csm g_prd cg
+  | LCsub  env #a #f csm prd cf csm' prd' prd_f          -> c_LCsub  a f csm prd cf csm' prd' prd_f
+
+
+(*** Semantics *)
+
+[@@ strict_on_arguments [5]] (* strict on [ct] *)
+let rec tree_req
+      (#env : vprop_list) (#a : Type u#a) (#t : M.prog_tree a) (#csm : csm_t env) (#prd : prd_t a)
+      (ct : lin_cond env t csm prd)
+      (sl0 : sl_f env)
+  : Tot Type0 (decreases ct)
+  = match ct with
+  | LCspec env #a #pre #post #req #ens csm_f ->
+      req (eij_sl (L.index csm_f) sl0)
+  | LCret  env #a #x #sl_hint prd csm_f ->
+      True
+  | LCbind env #a #b #f #g f_csm f_prd cf g_csm g_prd cg ->
+      tree_req cf sl0 /\
+      (forall (x : a) (sl_itm : sl_f (f_prd x)) .
+        tree_ens cf sl0 x sl_itm ==> tree_req (cg x) (res_sel sl0 f_csm sl_itm))
+  | LCsub  env #a #f csm prd cf csm' prd' prd_f ->
+      tree_req cf sl0
+
+and tree_ens
+      (#env : vprop_list) (#a : Type u#a) (#t : M.prog_tree a) (#csm : csm_t env) (#prd : prd_t a)
+      (ct : lin_cond env t csm prd)
+      (sl0 : sl_f env) (res : a) (sl1 : sl_f (prd res))
+  : Tot Type0 (decreases ct)
+  = match ct with
+  | LCspec env #a #pre #post #req #ens csm_f ->
+      ens (eij_sl (L.index csm_f) sl0) res sl1
+  | LCret  env #a #x #sl_hint prd csm_f ->
+      res == x /\ sl1 == eij_sl (L.index csm_f) sl0
+  | LCbind env #a #b #f #g f_csm f_prd cf g_csm g_prd cg ->
+      (exists (x : a) (sl_itm : sl_f (f_prd x)) .
+        tree_ens cf sl0 x sl_itm ==> tree_ens (cg x) (res_sel sl0 f_csm sl_itm) res sl1)
+  | LCsub  env #a #f csm prd cf csm' prd' prd_f ->
+      (exists (sl1' : sl_f (prd res)) . (
+        (**) Ll.pat_append ();
+        tree_ens cf sl0 res sl1' /\
+        sl1 == extract_vars (Perm.perm_f_of_list (prd_f res))
+          (Fl.append sl1' (filter_mask_fl csm' _
+                                (filter_mask_fl (mask_not csm) (vprop_list_sels_t env) sl0)))))
+
+
+(***** Equivalence *)
+
+let equiv' (#env : vprop_list) (#a : Type) (#t : M.prog_tree a) (#csm : csm_t env) (#prd : prd_t a)
+           (f g : lin_cond env t csm prd)
+  : prop
+  = (forall (sl0 : sl_f env) .
+       tree_req f sl0 <==> tree_req g sl0) /\
+    (forall (sl0 : sl_f env) . tree_req f sl0 ==>
+      (forall (res : a) (sl1 : sl_f (prd res)) .
+        tree_ens f sl0 res sl1 <==> tree_ens g sl0 res sl1))
+
+
+(*** Pushing [LCsub] to the leaves *)
+
+//[@@ strict_on_arguments [5]] (* strict on [ct] *)
+let rec lcsub_at_leaves
+      (#env : vprop_list) (#a : Type u#a) (#t : M.prog_tree a) (#csm : csm_t env) (#prd : prd_t a)
+      (ct : lin_cond env t csm prd)
+  : Tot prop (decreases ct)
+  = match ct with
+  | LCspec _ _ | LCret _ _ _ | LCsub  _ _ _ (LCspec _ _) _ _ _ ->
+           True
+  | LCbind _ #a _ _ cf _ _ cg ->
+           lcsub_at_leaves cf /\ (forall (x : a) . lcsub_at_leaves (cg x))
+  | LCsub  _ _ _ _ _ _ _ ->
+           False
+
+/// An alias to present a transformation
+type lcsubp_tr
+      (#env : vprop_list) (#a : Type) (#t : M.prog_tree a) (#csm : csm_t env) (#prd : prd_t a)
+      (f : lin_cond env t csm prd)
+  = lin_cond env t csm prd
+
+
+(***** [LCret] *)
+
+#push-options "--ifuel 0 --fuel 0"
+let sub_ret_prd_f'
+      (#env   : vprop_list)
+      (#prd0  : vprop_list) (csm_f0 : eq_injection_l prd0 env)
+      (#csm1  : csm_t (filter_mask (mask_not (eij_trg_mask csm_f0)) env)) (#prd1 : vprop_list)
+      (prd_f1 : vequiv_perm (sub_prd env (eij_trg_mask csm_f0) prd0 csm1) prd1)
+      (i : Fin.fin (L.length prd1))
+  : (j : Fin.fin (L.length env) {L.index env j == L.index prd1 i})
+  =
+    (**) Ll.pat_append ();
+    let n0    = L.length prd0 in
+    let ncsm0 = mask_not (eij_trg_mask csm_f0) in
+    let k = prd_f1 i in
+    (**) assert L.(index (prd0 @ (filter_mask csm1 (filter_mask ncsm0 env))) k == index prd1 i);
+    if k < n0
+    then begin
+      (**) assert L.(index prd0 k == index prd1 i);
+      L.index csm_f0 k
+    end else begin
+      (**) assert L.(index (filter_mask csm1 (filter_mask ncsm0 env)) (k - n0) == index prd1 i);
+      (mask_pull ncsm0 (mask_pull csm1 (k - n0)))
+    end
+
+val sub_ret_prd_f_eij
+      (#env   : vprop_list)
+      (#prd0  : vprop_list) (csm_f0 : eq_injection_l prd0 env)
+      (#csm1  : csm_t (filter_mask (mask_not (eij_trg_mask csm_f0)) env)) (#prd1 : vprop_list)
+      (prd_f1 : vequiv_perm (sub_prd env (eij_trg_mask csm_f0) prd0 csm1) prd1)
+  : Lemma (is_eq_injection prd1 env (sub_ret_prd_f' csm_f0 prd_f1))
+
+let sub_ret_prd_f
+      (#env   : vprop_list)
+      (#prd0  : vprop_list) (csm_f0 : eq_injection_l prd0 env)
+      (#csm1  : csm_t (filter_mask (mask_not (eij_trg_mask csm_f0)) env)) (#prd1 : vprop_list)
+      (prd_f1 : vequiv_perm (sub_prd env (eij_trg_mask csm_f0) prd0 csm1) prd1)
+  : eq_injection_l prd1 env
+  =
+    (**) sub_ret_prd_f_eij csm_f0 prd_f1;
+    Ll.initi 0 (L.length prd1) (sub_ret_prd_f' csm_f0 prd_f1)
+#pop-options
+
+val sub_ret_prd_f_eij_trg_eq
+      (#env   : vprop_list)
+      (#prd0  : vprop_list) (csm_f0 : eq_injection_l prd0 env)
+      (#csm1  : csm_t (filter_mask (mask_not (eij_trg_mask csm_f0)) env)) (#prd1 : vprop_list)
+      (prd_f1 : vequiv_perm (sub_prd env (eij_trg_mask csm_f0) prd0 csm1) prd1)
+  : Lemma (bind_csm env (eij_trg_mask csm_f0) csm1 == eij_trg_mask (sub_ret_prd_f csm_f0 (prd_f1)))
+
+let lcsubp_LCret
+      (env    : vprop_list) (a : Type u#a) (x : a) (sl_hint : M.post_t a)
+      (prd0   : prd_t a) (csm_f0 : eq_injection_l (prd0 x) env)
+      (csm1   : csm_t (filter_mask (mask_not (eij_trg_mask csm_f0)) env)) (prd1 : prd_t a)
+      (prd_f1 : (x' : a) -> Perm.pequiv_list (sub_prd env (eij_trg_mask csm_f0) (prd0 x') csm1) (prd1 x'))
+  : lcsubp_tr (LCsub env _ _ (LCret env #a #x #sl_hint prd0 csm_f0) csm1 prd1 prd_f1)
+  =
+    let prd_f1' : vequiv_perm (sub_prd env (eij_trg_mask csm_f0) (prd0 x) csm1) (prd1 x)
+                = Perm.perm_f_of_list (prd_f1 x) in
+    (**) sub_ret_prd_f_eij_trg_eq csm_f0 prd_f1';
+    LCret env #a #x #sl_hint prd1 (sub_ret_prd_f csm_f0 prd_f1')
+
+
+(***** [LCbind] *)
+
+let sub_bind_csm
+      (#env  : vprop_list)
+      (f_csm : csm_t env)
+      (g_csm : csm_t (filter_mask (mask_not f_csm) env))
+      (csm1  : csm_t (filter_mask (mask_not (bind_csm env f_csm g_csm)) env))
+  : csm_t (filter_mask (mask_not f_csm) env)
+  = mask_comp_or g_csm csm1
+
+#push-options "--ifuel 0 --fuel 0"
+let lcsubp_LCbind_prd_f
+      (#env   : vprop_list) (#b : Type u#a)
+      (f_csm  : csm_t env) (f_prd : vprop_list)
+      (g_csm  : csm_t (filter_mask (mask_not f_csm) env)) (g_prd : prd_t b)
+      (csm1   : csm_t (filter_mask (mask_not (bind_csm env f_csm g_csm)) env)) (prd1 : prd_t b)
+      (prd_f1 : (y : b) -> Perm.pequiv_list (sub_prd env (bind_csm env f_csm g_csm) (g_prd y) csm1) (prd1 y))
+      (y : b)
+  : Perm.pequiv_list
+      (sub_prd (res_env env f_csm f_prd) (bind_g_csm' env f_csm f_prd g_csm) (g_prd y) csm1) (prd1 y)  
+  =
+    (**) filter_bind_g_csm' env f_csm f_prd g_csm;
+    U.cast _ (prd_f1 y)
+
+type lcsubp_LCbind_rc_g
+      (env : vprop_list)
+      (a : Type u#a) (b : Type u#a) (g : a -> M.prog_tree b)
+      (f_csm : csm_t env) (f_prd : prd_t a)
+      (g_csm : csm_t (filter_mask (mask_not f_csm) env)) (g_prd : prd_t b)
+      (cg : (x : a) -> lin_cond (res_env env f_csm (f_prd x)) (g x) (bind_g_csm' env f_csm (f_prd x) g_csm) g_prd)
+      (csm1 : csm_t (filter_mask (mask_not (bind_csm env f_csm g_csm)) env)) (prd1 : prd_t b)
+      (prd_f1 : (y : b) -> Perm.pequiv_list (sub_prd env (bind_csm env f_csm g_csm) (g_prd y) csm1) (prd1 y))
+  = (x : a) -> lcsubp_tr (
+       LCsub (res_env env f_csm (f_prd x))
+             (bind_g_csm' env f_csm (f_prd x) g_csm) g_prd (cg x)
+             csm1 prd1 (lcsubp_LCbind_prd_f f_csm (f_prd x) g_csm g_prd csm1 prd1 prd_f1))
+
+let lcsubp_LCbind
+      (env : vprop_list)
+      (a : Type u#a) (b : Type u#a) (f : M.prog_tree a) (g : a -> M.prog_tree b)
+      (f_csm : csm_t env) (f_prd : prd_t a)
+      (cf : lin_cond env f f_csm f_prd)
+      (g_csm : csm_t (filter_mask (mask_not f_csm) env)) (g_prd : prd_t b)
+      (cg : (x : a) -> lin_cond (res_env env f_csm (f_prd x)) (g x) (bind_g_csm' env f_csm (f_prd x) g_csm) g_prd)
+      (csm1 : csm_t (filter_mask (mask_not (bind_csm env f_csm g_csm)) env)) (prd1 : prd_t b)
+      (prd_f1 : (y : b) -> Perm.pequiv_list (sub_prd env (bind_csm env f_csm g_csm) (g_prd y) csm1) (prd1 y))
+
+      (rc_f : lcsubp_tr cf)
+      (rc_g : lcsubp_LCbind_rc_g env a b g f_csm f_prd g_csm g_prd cg csm1 prd1 prd_f1)
+  : lcsubp_tr (LCsub env _ _ (LCbind env f_csm f_prd cf g_csm g_prd cg) csm1 prd1 prd_f1)
+  =
+    (**) mask_comp_or_assoc f_csm g_csm csm1;
+    LCbind env f_csm f_prd rc_f
+       (mask_comp_or g_csm csm1) prd1
+       (fun (x : a) ->
+         (**) bind_g_csm'_or env f_csm (f_prd x) g_csm csm1;
+         rc_g x)
+#pop-options
+
+
+(***** [LCsub] *)
+
+let comp_sub_csm
+      (#env : vprop_list)
+      (csm0 : csm_t env)
+      (csm1 : csm_t (filter_mask (mask_not csm0) env))
+      (csm2 : csm_t (filter_mask (mask_not (bind_csm env csm0 csm1)) env))
+  : csm_t (filter_mask (mask_not csm0) env)
+  = mask_comp_or csm1 csm2
+
+let bind_bind_csm
+      (#env : vprop_list)
+      (csm0 : csm_t env)
+      (csm1 : csm_t (filter_mask (mask_not csm0) env))
+      (csm2 : csm_t (filter_mask (mask_not (bind_csm env csm0 csm1)) env))
+  : Lemma (bind_csm env (bind_csm env csm0 csm1) csm2 == bind_csm env csm0 (comp_sub_csm csm0 csm1 csm2))
+          [SMTPat (bind_csm env (bind_csm env csm0 csm1) csm2)]
+  = mask_comp_or_assoc csm0 csm1 csm2
+
+#push-options "--ifuel 0 --fuel 0"
+let comp_sub_prd_f
+      (#env : vprop_list)
+      (#csm0 : csm_t env) (#prd0 : vprop_list)
+      (#csm1 : csm_t (filter_mask (mask_not csm0) env)) (#prd1 : vprop_list)
+      (#csm2 : csm_t (filter_mask (mask_not (bind_csm env csm0 csm1)) env)) (#prd2 : vprop_list)
+      (f1 : Perm.pequiv_list (sub_prd env csm0 prd0 csm1) prd1)
+      (f2 : Perm.pequiv_list (sub_prd env (bind_csm env csm0 csm1) prd1 csm2) prd2)
+  : Perm.pequiv_list (sub_prd env csm0 prd0 (comp_sub_csm csm0 csm1 csm2)) prd2
+  = 
+    let f1 : vequiv_perm (sub_prd env csm0 prd0 csm1) prd1 = Perm.perm_f_of_list f1                     in
+    let f2 : vequiv_perm (sub_prd env (bind_csm env csm0 csm1) prd1 csm2) prd2 = Perm.perm_f_of_list f2 in
+    let env1  = filter_mask (mask_not csm0) env                     in
+    let flt1  = filter_mask csm1 env1                               in
+    let flt2  = filter_mask csm2 (filter_mask (mask_not csm1) env1) in
+    let flt12 = filter_mask (mask_comp_or csm1 csm2) env1           in
+
+    assert (sub_prd env csm0 prd0 csm1 == L.(prd0 @ flt1));
+    calc (==) {
+      sub_prd env (bind_csm env csm0 csm1) prd1 csm2;
+    == { }
+      L.(prd1 @ (filter_mask csm2 (filter_mask (mask_not (mask_comp_or csm0 csm1)) env)));
+    == { mask_not_comp_or csm0 csm1;
+         filter_mask_and (mask_not csm0) (mask_not csm1) env }
+      L.(prd1 @ flt2);
+    };
+    assert (sub_prd env csm0 prd0 (comp_sub_csm csm0 csm1 csm2) == L.(prd0 @ flt12));
+
+    let f1 : vequiv_perm L.(prd0 @ flt1) prd1 = U.cast _ f1 in
+    let f2 : vequiv_perm L.(prd1 @ flt2) prd2 = U.cast _ f2 in
+    (**) filter_mask_or_append csm1 csm2 env1;
+    let eq_flt_or
+      : vequiv_perm flt12 L.(flt1 @ flt2)
+      = U.cast (Perm.perm_f (L.length flt12)) (mask_or_append_f csm1 csm2)
+    in
+    (**) L.append_assoc prd0 flt1 flt2;
+    let f3 : vequiv_perm L.(prd0 @ flt1 @ flt2) prd2
+      = U.cast _ Perm.(pequiv_trans (pequiv_append f1 (pequiv_refl _)) f2) in
+    let f4 : vequiv_perm (sub_prd env csm0 prd0 (comp_sub_csm csm0 csm1 csm2)) prd2
+      = U.cast _ Perm.(pequiv_trans (pequiv_append (pequiv_refl prd0) eq_flt_or) f3) in
+    Perm.perm_f_to_list f4
+#pop-options
+
+let lcsubp_LCsub
+      (env : vprop_list) (a : Type u#a) (f : M.prog_tree a)
+      (csm0 : csm_t env) (prd0 : prd_t a)
+      (cf : lin_cond env f csm0 prd0)
+      (csm1 : csm_t (filter_mask (mask_not csm0) env)) (prd1 : prd_t a)
+      (prd_f1 : (x : a) -> Perm.pequiv_list (sub_prd env csm0 (prd0 x) csm1) (prd1 x))
+      (csm2 : csm_t (filter_mask (mask_not (bind_csm env csm0 csm1)) env)) (prd2 : prd_t a)
+      (prd_f2 : (x : a) -> Perm.pequiv_list (sub_prd env (bind_csm env csm0 csm1) (prd1 x) csm2) (prd2 x))
+
+      (rc_g : lcsubp_tr (LCsub env csm0 prd0 cf (comp_sub_csm csm0 csm1 csm2) prd2
+                                    (fun x -> comp_sub_prd_f (prd_f1 x) (prd_f2 x))))
+  : lcsubp_tr (LCsub env _ _ (LCsub env csm0 prd0 cf csm1 prd1 prd_f1) csm2 prd2 prd_f2)
+  = rc_g
+
+/// We could prove that this transformation yields an equivalent program ([equiv]) but it is not necessary to prove it.
+(*
+val lcsubp_LCsub
+      (#env : vprop_list) (#a : Type u#a) (#f : M.prog_tree a)
+      (#csm0 : csm_t env) (#prd0 : prd_t a)
+      (cf : lin_cond env f csm0 prd0)
+      (csm1 : csm_t (filter_mask (mask_not csm0) env)) (prd1 : prd_t a)
+      (prd_f1 : (x : a) -> vequiv_perm (sub_prd env csm0 (prd0 x) csm1) (prd1 x))
+      (csm2 : csm_t (filter_mask (mask_not (bind_csm env csm0 csm1)) env)) (prd2 : prd_t a)
+      (prd_f2 : (x : a) -> vequiv_perm (sub_prd env (bind_csm env csm0 csm1) (prd1 x) csm2) (prd2 x))
+  : equiv'
+      (LCsub env _ _ (LCsub env csm0 prd0 cf csm1 prd1 prd_f1) csm2 prd2 prd_f2)
+      (LCsub env csm0 prd0 cf (comp_sub_csm csm0 csm1 csm2) prd2 (fun x -> comp_sub_prd_f (prd_f1 x) (prd_f2 x)))
+*)
+
+(**** Definition of the transformation *)
+
+(* Since we use F* binders for LCbind, we cannot define a size like this
+let rec lin_cond_size
+      (#env : vprop_list) (#a : Type u#a) (#t : M.prog_tree a) (#csm : csm_t env) (#prd : prd_t a)
+      (lc : lin_cond env t csm prd)
+  : Tot nat (decreases lc)
+  = match lc with
+  | LCspec _ _ | LCret  _ _ _ -> 0
+  | LCbind _ _ _ cf _ _ cg -> lin_cond_size cf + lin_cond_size cg + 1
+  | LCsub  _ _ _ cf _ _ _ -> lin_cond cf + 1
+*)
+
+#push-options "--ifuel 1 --fuel 0 --z3rlimit 20"
+(**) private val ___begin_lc_sub_push : unit
+
+[@@ strict_on_arguments [5]] (* strict on [ct] *)
+let rec lc_sub_push
+      (#env : vprop_list) (#a : Type u#a) (#t : M.prog_tree a) (#csm : csm_t env) (#prd : prd_t a)
+      (ct : lin_cond env t csm prd)
+  : Tot (lcsubp_tr ct) (decreases %[ct; 1])
+  = match ct with
+  | LCspec _ _ | LCret  _ _ _ -> ct
+  | LCbind env f_csm f_prd cf g_csm g_prd cg ->
+      LCbind env f_csm f_prd (lc_sub_push cf) g_csm g_prd (fun x -> lc_sub_push (cg x))
+  | LCsub  env csm prd cf csm' prd' prd_f ->
+      lc_sub_push_aux cf csm' prd' prd_f
+
+and lc_sub_push_aux
+      (#env : vprop_list) (#a : Type u#a) (#t : M.prog_tree a) (#csm : csm_t env) (#prd : prd_t a)
+      (ct : lin_cond env t csm prd)
+      (csm' : csm_t (filter_mask (mask_not csm) env)) (prd' : prd_t a)
+      (prd_f : ((x : a) -> Perm.pequiv_list (sub_prd env csm (prd x) csm') (prd' x)))
+  : Tot (lcsubp_tr (LCsub env _ _ ct csm' prd' prd_f)) (decreases %[ct; 0])
+  = match ct with
+  | LCspec _ _ ->
+      LCsub _ _ _ ct csm' prd' prd_f
+  | LCret  _ #a #x #sl_hint prd0 csm_f0 ->
+      lcsubp_LCret env a x sl_hint prd0 csm_f0 csm' prd'
+        (fun (x' : a) -> U.cast #(Perm.pequiv_list (sub_prd env csm (prd x') csm') (prd' x')) _ (prd_f x'))
+  | LCbind env #a #b #f #g f_csm f_prd cf g_csm g_prd cg ->
+      let csm1 : csm_t (filter_mask (mask_not (bind_csm env f_csm g_csm)) env) = csm' in
+      let prd1 : prd_t b = prd' in
+      let prd_f1 (y : b) : Perm.pequiv_list (sub_prd env (bind_csm env f_csm g_csm) (g_prd y) csm1) (prd1 y)
+             = U.cast _ (prd_f y) in
+      let rc_f : lcsubp_tr cf = lc_sub_push cf in
+      let rc_g : lcsubp_LCbind_rc_g env a b g f_csm f_prd g_csm g_prd cg csm1 prd1 prd_f1
+        = fun (x : a) ->
+           let env'   = res_env env f_csm (f_prd x) in
+           let g_csm' = bind_g_csm' env f_csm (f_prd x) g_csm in
+           let cg   : lin_cond env' (g x) g_csm' g_prd = cg x in
+           (**) filter_bind_g_csm' env f_csm (f_prd x) g_csm;
+           let csm1 : csm_t (filter_mask (mask_not g_csm') env') = csm1 in
+           lc_sub_push_aux
+             #env' #b #(g x)
+             #g_csm' #g_prd cg
+             csm1 prd1
+             (lcsubp_LCbind_prd_f f_csm (f_prd x) g_csm g_prd csm1 prd1 prd_f1)
+      in
+      lcsubp_LCbind env a b f g f_csm f_prd cf g_csm g_prd cg csm1 prd1 prd_f1 rc_f rc_g
+  | LCsub  env #a #f csm0 prd0 cf csm1 prd1 prd_f1 ->
+      let csm2 : csm_t (filter_mask (mask_not (bind_csm env csm0 csm1)) env) = csm' in
+      let prd2 : prd_t a = prd' in
+      let prd_f2 (x : a) : Perm.pequiv_list (sub_prd env (bind_csm env csm0 csm1) (prd1 x) csm2) (prd2 x)
+               = U.cast _ (prd_f x) in
+      let prd_f' (x : a) = comp_sub_prd_f (prd_f1 x) (prd_f2 x) in
+      let rc : lcsubp_tr (LCsub env csm0 prd0 cf (comp_sub_csm csm0 csm1 csm2) prd2 prd_f')
+        = lc_sub_push_aux #env #a #f #csm0 #prd0 cf (comp_sub_csm csm0 csm1 csm2) prd2 prd_f'
+      in
+      lcsubp_LCsub env a f csm0 prd0 cf csm1 prd1 prd_f1 csm2 prd2 prd_f2 rc
+#pop-options
+
+
+val lc_sub_push_at_leaves
+      (env : vprop_list) (#a : Type u#a) (#t : M.prog_tree a) (#csm : csm_t env) (#prd : prd_t a)
+      (ct : lin_cond env t csm prd)
+  : Lemma (lcsub_at_leaves (lc_sub_push ct))
